src/Parsers/ContextFreeGrammarProperties.v
@@ -1,4 +1,5 @@
 (** * Properties about Context Free Grammars *)
+Require Import Coq.Strings.String.
 Require Import Parsers.StringLike Parsers.ContextFreeGrammar.
 
 Set Implicit Arguments.
@@ -7,7 +8,16 @@ Delimit Scope string_like_scope with string_like.
 
 Section cfg.
   Context CharType (String : string_like CharType) (G : grammar CharType)
-          (P : productions CharType -> Type).
+          (P : string -> Type).
+
+  Definition Forall_parse_of_item'
+             (Forall_parse_of : forall {str pats} (p : parse_of String G str pats), Type)
+             {str it} (p : parse_of_item String G str it)
+    := match p return Type with
+         | ParseTerminal x => unit
+         | ParseNonTerminal name str p'
+           => (P name * Forall_parse_of p')%type
+       end.
 
   Fixpoint Forall_parse_of {str pats} (p : parse_of String G str pats)
     := match p with
@@ -17,22 +27,12 @@ Section cfg.
            => Forall_parse_of p'
        end
   with Forall_parse_of_production {str pat} (p : parse_of_production String G str pat)
-       := let Forall_parse_of_item {str it} (p : parse_of_item String G str it)
-              := match p return Type with
-                   | ParseTerminal x => unit
-                   | ParseNonTerminal name str p'
-                     => (P (Lookup G name) * Forall_parse_of p')%type
-                 end in
-          match p return Type with
+       := match p return Type with
             | ParseProductionNil => unit
             | ParseProductionCons str pat strs pats p' p''
-              => (Forall_parse_of_item p' * Forall_parse_of_production p'')%type
+              => (Forall_parse_of_item' (@Forall_parse_of) p' * Forall_parse_of_production p'')%type
           end.
 
   Definition Forall_parse_of_item {str it} (p : parse_of_item String G str it)
-    := match p return Type with
-         | ParseTerminal x => unit
-         | ParseNonTerminal name str p'
-           => (P (Lookup G name) * Forall_parse_of p')%type
-       end.
+    := @Forall_parse_of_item' (@Forall_parse_of) str it p.
 End cfg.
